code/experimental/P256/Hacl.Spec.P256.MontgomeryMultiplication.PointAdd.fst
@@ -19,79 +19,8 @@ let prime = prime256
 
 #reset-options "--z3rlimit 500"  
 
-
-val lemma_xToSpecification: 
-  x1D: nat -> y1D: nat -> z1D: nat -> x2D: nat -> y2D: nat -> z2D: nat -> 
-  
-  u1: nat{u1 = toDomain_ (z2D * z2D * x1D % prime)} -> 
-  u2: nat{u2 = toDomain_ (z1D * z1D * x2D % prime)} -> 
-  
-  s1: nat{s1 = toDomain_ (z2D * z2D * z2D * y1D % prime)} -> 
-  s2: nat{s2 = toDomain_ (z1D * z1D * z1D * y2D % prime)} ->
-
-  x3: nat{ 
-    let u1D, u2D = fromDomain_ u1, fromDomain_ u2 in 
-    let s1D, s2D = fromDomain_ s1, fromDomain_ s2 in  
-    (u1D = u2D && s1D = s2D && z1D <> 0 && z2D <> 0) ==> 
-      (let (xN, yN, zN) = _point_double (x1D, y1D, z1D) in fromDomain_ x3 == xN)} -> 
-   y3: nat{
-    let u1D, u2D = fromDomain_ u1, fromDomain_ u2 in 
-    let s1D, s2D = fromDomain_ s1, fromDomain_ s2 in  
-    (u1D = u2D && s1D = s2D && z1D <> 0 && z2D <> 0) ==> 
-      (let (xN, yN, zN) = _point_double (x1D, y1D, z1D) in fromDomain_ y3 == yN)} ->
-   z3: nat{
-     let u1D, u2D = fromDomain_ u1, fromDomain_ u2 in 
-     let s1D, s2D = fromDomain_ s1, fromDomain_ s2 in  
-     (u1D = u2D && s1D = s2D && z1D <> 0 && z2D <> 0) ==>
-       (let (xN, yN, zN) = _point_double (x1D, y1D, z1D) in fromDomain_ z3 == zN)}
-  ->  
-  Lemma 
-  (    
-    let (xN, yN, zN) = _point_add (x1D, y1D, z1D) (x2D, y2D, z2D) in
-    let x3D, y3D, z3D = fromDomainPoint (x3,  y3,  z3) in 
-    let u1D = fromDomain_ u1 in let u2D = fromDomain_ u2 in 
-    let s1D = fromDomain_ s1 in let s2D = fromDomain_ s2 in 
-    (u1D = u2D && s1D = s2D && z1D <> 0 && z2D <> 0)  ==> (xN == x3D /\ yN == y3D /\ zN == z3D)
-  )
-
-
-let lemma_xToSpecification x1D y1D z1D x2D y2D z2D u1 u2 s1 s2  x3 y3 z3 = 
-    let open FStar.Tactics in 
-    let open FStar.Tactics.Canon in 
-    let u1D = fromDomain_ u1 in let u2D = fromDomain_ u2 in 
-    let s1D = fromDomain_ s1 in let s2D = fromDomain_ s2 in  
-    
-    let (xN, yN, zN) = _point_add (x1D, y1D, z1D) (x2D, y2D, z2D) in 
-    let (xDouble, yDouble, zDouble) = _point_double (x1D, y1D, z1D) in 
-
-    let u1N = x1D * z2D * z2D % prime in 
-    let u2N = x2D * z1D * z1D % prime in 
-    let s1N = y1D * z2D * z2D * z2D % prime in 
-    let s2N = y2D * z1D * z1D * z1D % prime in 
-
-    assert_by_tactic (x1D * z2D * z2D = x1D * (z2D * z2D)) canon;
-    assert_by_tactic (x2D * z1D * z1D = x2D * (z1D * z1D)) canon;
-    
-    assert_by_tactic (y1D * z2D * (z2D * z2D) = y1D * z2D * z2D * z2D) canon;
-    assert_by_tactic (y2D * z1D * (z1D * z1D) = y2D * z1D * z1D * z1D) canon;
-
-    assert_by_tactic (z2D * z2D * z2D * y1D = y1D * z2D * z2D * z2D) canon;
-    assert_by_tactic (z1D * z1D * z1D * y2D = y2D * z1D * z1D * z1D) canon;
-
-
-     lemmaToDomainAndBackIsTheSame (u1N);
-     lemmaToDomainAndBackIsTheSame (u2N);
-     lemmaToDomainAndBackIsTheSame (s1N);
-     lemmaToDomainAndBackIsTheSame (s2N);
-
-    assert(u1N == u1D);
-    assert(u2N == u2D);
-    assert(s1N == s1D);
-    assert(s2N == s2D)
-
-     
 noextract       
-val lemma_xToSpecification_after_double: 
+val lemma_pointAddToSpecification: 
   pxD: nat -> pyD: nat -> pzD: nat -> 
   qxD: nat -> qyD: nat -> qzD: nat -> 
   x3: nat -> y3: nat -> z3: nat -> 
@@ -113,20 +42,16 @@ val lemma_xToSpecification_after_double:
       
       h == toDomain_ ((u2D - u1D) % prime256) /\
       r == toDomain_ ((s2D - s1D) % prime256) /\
-
       (
-	if (not (fromDomain_ u1 = fromDomain_ u2 && fromDomain_ s1 = fromDomain_ s2 && pzD <> 0 && qzD <> 0)) then 
-	(
-	  if qzD = 0 then 
-	    fromDomain_ x3 == pxD /\ fromDomain_ y3 == pyD /\ fromDomain_ z3 == pzD
-	  else if pzD = 0 then 
+	if qzD = 0 then 
+	  fromDomain_ x3 == pxD /\ fromDomain_ y3 == pyD /\ fromDomain_ z3 == pzD
+	else if pzD = 0 then 
 	    fromDomain_ x3 == qxD /\  fromDomain_ y3 == qyD /\  fromDomain_ z3 == qzD 
-	  else
+	else
 	    x3 == toDomain_ ((rD * rD - hD * hD * hD - 2 * hD * hD * u1D) % prime) /\
 	    y3 == toDomain_ (((hD * hD * u1D - x3D) * rD - s1D * hD*hD*hD) % prime) /\
 	    z3 == toDomain_ ((pzD * qzD * hD) % prime)
 	)
-	else True)
       )
   )
   (ensures 
@@ -135,14 +60,12 @@ val lemma_xToSpecification_after_double:
     let (xN, yN, zN) = _point_add (pxD, pyD, pzD) (qxD, qyD, qzD) in
     let u1D = fromDomain_ u1 in let u2D = fromDomain_ u2 in 
     let s1D = fromDomain_ s1 in let s2D = fromDomain_ s2 in 
-    if (not(u1D = u2D && s1D = s2D && pzD <> 0 && qzD <> 0)) then
-      xN == x3D /\  yN == y3D /\ zN == z3D
-    else True
+    xN == x3D /\  yN == y3D /\ zN == z3D
   )
 )
 
 
-let lemma_xToSpecification_after_double x1D y1D z1D x2D y2D z2D x3 y3 z3  u1 u2 s1 s2 h r = 
+let lemma_pointAddToSpecification x1D y1D z1D x2D y2D z2D x3 y3 z3  u1 u2 s1 s2 h r = 
     let open FStar.Tactics in 
     let open FStar.Tactics.Canon in 
     
